Finished consistent_waits and working on unique_crs

ConsistentWaits.v
@@ -1,67 +1,84 @@
 From Elo Require Import Core.
 
 From Elo Require Import NoCR.
-From Elo Require Import ValidTerm.
-From Elo Require Import NoWaits.
-From Elo Require Import ReservedWaits.
-From Elo Require Import ValidWaits.
+From Elo Require Import Keywords.
 
 (* ------------------------------------------------------------------------- *)
 (* consistent-waits                                                          *)
 (* ------------------------------------------------------------------------- *)
 
-Inductive consistent_waits (o : option addr) : tm -> Prop :=
-  | cwaits_unit  :                  consistent_waits o <{unit              }>
-  | cwaits_nat   : forall n,        consistent_waits o <{nat n             }>
-  | cwaits_plus  : forall t1 t2,    consistent_waits o t1 ->
-                                    consistent_waits o t2 ->
-                                    consistent_waits o <{t1 + t2           }>
-  | cwaits_monus : forall t1 t2,    consistent_waits o t1 ->
-                                    consistent_waits o t2 ->
-                                    consistent_waits o <{t1 - t2           }>
-  | cwaits_seq   : forall t1 t2,    consistent_waits o t1 ->
-                                    consistent_waits o t2 ->
-                                    consistent_waits o <{t1; t2            }>
-  | cwaits_if    : forall t1 t2 t3, consistent_waits o t1 ->
-                                    consistent_waits o t2 ->
-                                    consistent_waits o t3 ->
-                                    consistent_waits o (tm_if t1 t2 t3     )
-  | cwaits_while : forall t1 t2,    consistent_waits o t1 ->
-                                    consistent_waits o t2 ->
-                                    consistent_waits o <{while t1 do t2 end}>
-  | cwaits_var   : forall x,        consistent_waits o <{var x             }>
-  | cwaits_fun   : forall x Tx t,   consistent_waits o t  ->
-                                    consistent_waits o <{fn x Tx t         }>
-  | cwaits_call  : forall t1 t2,    consistent_waits o t1 ->
-                                    consistent_waits o t2 ->
-                                    consistent_waits o <{call t1 t2        }>
-  | cwaits_ref   : forall ad T,     consistent_waits o <{&ad : T           }>
-  | cwaits_new   : forall t T,      consistent_waits o t  ->
-                                    consistent_waits o <{new t : T         }>
-  | cwaits_init  : forall ad t T,   consistent_waits o t  ->
-                                    consistent_waits o <{init ad t : T     }>
-  | cwaits_load  : forall t,        consistent_waits o t  ->
-                                    consistent_waits o <{*t                }>
-  | cwaits_asg   : forall t1 t2,    consistent_waits o t1 ->
-                                    consistent_waits o t2 ->
-                                    consistent_waits o <{t1 := t2          }>
-  | cwaits_acq   : forall t1 x t2,  consistent_waits o t1 ->
-                                    reserved_waits t2     ->
-                                    consistent_waits o <{acq t1 x t2       }>
-  | cwaits_cr    : forall ad t,     consistent_waits (Some ad) t ->
-                                    consistent_waits o <{cr ad t           }>
-  | cwaits_wait1 :                  o = None    ->
-                                    consistent_waits o <{wait (var SELF)   }>
-  | cwaits_wait2 : forall ad T,     o = Some ad ->
-                                    consistent_waits o <{wait (&ad : T)    }>
-  | cwaits_reacq : forall ad,       consistent_waits o <{reacq ad          }>
-  | cwaits_spawn : forall t,        consistent_waits None t ->
-                                    consistent_waits o <{spawn t           }>
+Inductive wait_region : Set :=
+  | WR_none
+  | WR_self
+  | WR_ad : addr -> wait_region
+  .
+
+(*
+  (!!!) consistent_waits is an initial condition.
+  (!!!) consistent_waits is an invariant.
+
+  - WR_none  => no  immediate* waits.
+  - WR_self  => any immediate* wait is a wait with SELF.
+  - WR_ad ad => any immediate* wait is a wait with the given address.
+  (waits are immediate if they do not appear inside fun/acq/cr/spawn blocks.)
+
+  - fun   blocks are WR_none.
+  - acq   blocks are WR_self.
+  - cr ad blocks are (WR_ad ad).
+  - spawn blocks are WR_none.
+*)
+Inductive consistent_waits: wait_region -> tm -> Prop :=
+  | cw_unit  : forall WR,          consistent_waits WR <{unit              }>
+  | cw_nat   : forall WR n,        consistent_waits WR <{nat n             }>
+  | cw_plus  : forall WR t1 t2,    consistent_waits WR t1 ->
+                                   consistent_waits WR t2 ->
+                                   consistent_waits WR <{t1 + t2           }>
+  | cw_monus : forall WR t1 t2,    consistent_waits WR t1 ->
+                                   consistent_waits WR t2 ->
+                                   consistent_waits WR <{t1 - t2           }>
+  | cw_seq   : forall WR t1 t2,    consistent_waits WR t1 ->
+                                   consistent_waits WR t2 ->
+                                   consistent_waits WR <{t1; t2            }>
+  | cw_if    : forall WR t1 t2 t3, consistent_waits WR t1 ->
+                                   consistent_waits WR t2 ->
+                                   consistent_waits WR t3 ->
+                                   consistent_waits WR (tm_if t1 t2 t3     )
+  | cw_while : forall WR t1 t2,    consistent_waits WR t1 ->
+                                   consistent_waits WR t2 ->
+                                   consistent_waits WR <{while t1 do t2 end}>
+  | cw_var   : forall WR x,        consistent_waits WR <{var x             }>
+  | cw_fun   : forall WR x Tx t,   consistent_waits WR_none t  ->
+                                   consistent_waits WR <{fn x Tx t         }>
+  | cw_call  : forall WR t1 t2,    consistent_waits WR t1 ->
+                                   consistent_waits WR t2 ->
+                                   consistent_waits WR <{call t1 t2        }>
+  | cw_ref   : forall WR ad T,     consistent_waits WR <{&ad : T           }>
+  | cw_new   : forall WR t T,      consistent_waits WR t  ->
+                                   consistent_waits WR <{new t : T         }>
+  | cw_init  : forall WR ad t T,   consistent_waits WR t  ->
+                                   consistent_waits WR <{init ad t : T     }>
+  | cw_load  : forall WR t,        consistent_waits WR t  ->
+                                   consistent_waits WR <{*t                }>
+  | cw_asg   : forall WR t1 t2,    consistent_waits WR t1 ->
+                                   consistent_waits WR t2 ->
+                                   consistent_waits WR <{t1 := t2          }>
+  | cw_acq   : forall WR t1 x t2,  consistent_waits WR t1        ->
+                                   consistent_waits (WR_self) t2 ->
+                                   consistent_waits WR <{acq t1 x t2       }>
+  | cw_cr    : forall WR ad t,     consistent_waits (WR_ad ad) t ->
+                                   consistent_waits WR <{cr ad t           }>
+
+  | cw_wait1 :                   consistent_waits WR_self    <{wait (var SELF)}>
+  | cw_wait2 : forall ad T,      consistent_waits (WR_ad ad) <{wait (&ad : T) }>
+
+  | cw_reacq : forall WR ad,       consistent_waits WR <{reacq ad          }>
+  | cw_spawn : forall WR t,        consistent_waits (WR_none) t ->
+                                   consistent_waits WR <{spawn t           }>
   .
 
 (* inversion --------------------------------------------------------------- *)
 
-Local Ltac _cwaits tt :=
+Local Ltac _cw tt :=
   match goal with
   | H : consistent_waits _ <{unit                  }> |- _ => clear H
   | H : consistent_waits _ <{nat _                 }> |- _ => clear H
@@ -70,7 +87,7 @@ Local Ltac _cwaits tt :=
   | H : consistent_waits _ <{_; _                  }> |- _ => tt H
   | H : consistent_waits _ <{if _ then _ else _ end}> |- _ => tt H
   | H : consistent_waits _ <{while _ do _ end      }> |- _ => tt H
-  | H : consistent_waits _ <{var _                 }> |- _ => tt H
+  | H : consistent_waits _ <{var _                 }> |- _ => clear H
   | H : consistent_waits _ <{fn _ _ _              }> |- _ => tt H
   | H : consistent_waits _ <{call _ _              }> |- _ => tt H
   | H : consistent_waits _ <{&_ : _                }> |- _ => clear H
@@ -85,170 +102,254 @@ Local Ltac _cwaits tt :=
   | H : consistent_waits _ <{spawn _               }> |- _ => tt H
   end.
 
-Ltac inv_cwaits  := _cwaits inv.
-Ltac invc_cwaits := _cwaits invc.
+Ltac inv_cw  := _cw inv.
+Ltac invc_cw := _cw invc.
 
 (* lemmas ------------------------------------------------------------------ *)
 
-Lemma cwaits_from_nowaits : forall o t,
-  no_waits t ->
-  consistent_waits o t.
+Lemma wrself_from_wrnone : forall t,
+  consistent_waits WR_none t ->
+  consistent_waits WR_self t.
 Proof.
-  intros. gendep o. induction t; intros; invc_nowaits;
-  auto using rwaits_from_nowaits, consistent_waits.
+  intros. induction t; invc_cw; auto using consistent_waits. 
 Qed.
 
-Lemma cwaits_from_rwaits : forall t,
-  no_crs t ->
-  (* --- *)
-  reserved_waits t ->
-  consistent_waits None t.
+Lemma wrad_from_wrnone : forall ad t,
+  consistent_waits WR_none t ->
+  consistent_waits (WR_ad ad) t.
 Proof.
-  intros. induction t; invc_nocrs; invc_rwaits; auto using consistent_waits.
+  intros. induction t; invc_cw; auto using consistent_waits. 
+Qed.
+
+Lemma wrnone_weakening : forall o t,
+  value t ->
+  (* --- *)
+  consistent_waits o t ->
+  consistent_waits WR_none t.
+Proof.
+  intros * Hval ?. invc Hval; invc_cw; auto using consistent_waits. 
+Qed.
+
+Lemma wrnone_strengthening : forall o t,
+  consistent_waits WR_none t ->
+  consistent_waits o t.
+Proof.
+  intros. induction t; invc_cw; auto using consistent_waits. 
+Qed.
+
+Lemma wrad_strengthening : forall o ad t,
+  value t ->
+  (* --- *)
+  consistent_waits (WR_ad ad) t ->
+  consistent_waits o t.
+Proof.
+  intros * Hval ?. invc Hval; invc_cw; auto using consistent_waits.
+Qed.
+
+Lemma wrnone_init_term : forall o t1 t2 ad' t',
+  consistent_waits o t1 ->
+  t1 --[e_init ad' t']--> t2   ->
+  consistent_waits WR_none t'.
+Proof.
+  intros. gendep o; ind_tstep; intros; invc_cw;
+  eauto using wrnone_weakening, consistent_waits.
+Qed.
+
+Lemma wrnone_write_term : forall o t1 t2 ad' t',
+  consistent_waits o t1 ->
+  t1 --[e_write ad' t']--> t2   ->
+  consistent_waits WR_none t'.
+Proof.
+  intros. gendep o; ind_tstep; intros; invc_cw;
+  eauto using wrnone_weakening, consistent_waits.
 Qed.
 
 (* preservation lemmas ----------------------------------------------------- *)
 
-Lemma cwaits_subst : forall t ad T,
-  no_crs t      ->
-  valid_waits t ->
-  (* --- *)
-  reserved_waits t ->
-  consistent_waits (Some ad) <{[SELF := &ad : T] t}>.
+Lemma wrnone_subst : forall x tx t,
+  consistent_waits WR_none t  ->
+  consistent_waits WR_none tx ->
+  consistent_waits WR_none <{[x := tx] t}>
+with wrself_subst : forall x tx t,
+  x <> SELF ->
+  consistent_waits WR_self t ->
+  consistent_waits WR_none tx ->
+  consistent_waits WR_self <{[x := tx] t}>
+with wrad_subst  : forall ad x tx t,
+  consistent_waits (WR_ad ad) t ->
+  consistent_waits WR_none tx ->
+  consistent_waits (WR_ad ad) <{[x := tx] t}>.
 Proof.
-  intros. induction t; invc_nocrs; invc_vwaits; invc_rwaits;
+  all: intros; induction t; invc_cw; simpl; repeat destruct _str_eq_dec;
+       auto using wrself_from_wrnone, wrad_from_wrnone, consistent_waits.
+Qed.
+
+Lemma cw_subst : forall o x tx t,
+  value tx ->
+  (* --- *)
+  x <> SELF             ->
+  consistent_waits o t  ->
+  consistent_waits o tx ->
+  consistent_waits o <{[x := tx] t}>.
+Proof.
+  intros. gendep o. induction t; intros; inv_cw;
+  simpl; repeat destruct _str_eq_dec; auto using consistent_waits;
+  eauto using wrnone_weakening, consistent_waits, wrself_subst, wrad_subst.
+Qed.
+
+Lemma wrnone_subst_self : forall t ad T,
+  consistent_waits WR_none t ->
+  consistent_waits WR_none <{[SELF := (&ad : T)] t}>
+with wrad_subst_self : forall t ad ad' T,
+  consistent_waits (WR_ad ad') t ->
+  consistent_waits (WR_ad ad') <{[SELF := (&ad : T)] t}>.
+Proof.
+  - intros. induction t; invc_cw;
+    remember SELF as x; simpl; repeat destruct _str_eq_dec; subst;
+    auto using consistent_waits.
+  - intros. induction t; invc_cw;
+    remember SELF as x; simpl; repeat destruct _str_eq_dec; subst;
+    auto using consistent_waits.
+Qed.
+
+Lemma cw_subst_self : forall t ad T,
+  consistent_waits WR_self t ->
+  consistent_waits (WR_ad ad) <{[SELF := (&ad : T)] t}>.
+Proof.
+  intros. induction t; invc_cw;
   remember SELF as x; simpl; repeat destruct _str_eq_dec; subst;
-  auto using cwaits_from_rwaits, consistent_waits.
+  auto using wrnone_subst_self, wrad_subst_self, consistent_waits.
 Qed.
 
 (* preservation ------------------------------------------------------------ *)
 
-Local Ltac solve_cwaits_preservation :=
+Local Ltac solve_cw_preservation :=
   intros o **; gendep o; ind_tstep; intros;
-  repeat invc_vtm; repeat invc_vwaits; repeat invc_cwaits; repeat constructor;
-  auto using nowaits_from_value, nowaits_subst, cwaits_from_nowaits.
+  repeat invc_kw; repeat invc_cw; repeat constructor; auto;
+  eauto using wrnone_strengthening, wrad_strengthening,
+             cw_subst, cw_subst_self,
+             consistent_waits.
 
-Lemma cwaits_preservation_none : forall o t1 t2,
-  valid_waits t1 ->
+Lemma cw_preservation_none : forall o t1 t2,
+  keywords t1 ->
   (* --- *)
   consistent_waits o t1 ->
-  t1 --[e_none]--> t2 ->
+  t1 --[e_none]--> t2   ->
   consistent_waits o t2.
-Proof. solve_cwaits_preservation. Qed.
+Proof. solve_cw_preservation. Qed.
 
-Lemma cwaits_preservation_alloc : forall o t1 t2 ad' T',
-  consistent_waits o t1 ->
+Lemma cw_preservation_alloc : forall o t1 t2 ad' T',
+  consistent_waits o t1       ->
   t1 --[e_alloc ad' T']--> t2 ->
   consistent_waits o t2.
-Proof. solve_cwaits_preservation. Qed.
+Proof. solve_cw_preservation. Qed.
 
-Lemma cwaits_preservation_init : forall o t1 t2 ad' t',
-  consistent_waits o t1 ->
+Lemma cw_preservation_init : forall o t1 t2 ad' t',
+  consistent_waits o t1      ->
   t1 --[e_init ad' t']--> t2 ->
   consistent_waits o t2.
-Proof. solve_cwaits_preservation. Qed.
+Proof. solve_cw_preservation. Qed.
 
-Lemma cwaits_preservation_read : forall o t1 t2 ad' t',
-  value t'       ->
-  valid_waits t' ->
+Lemma cw_preservation_read : forall o t1 t2 ad' t',
+  value t'                    ->
+  consistent_waits WR_none t' ->
   (* --- *)
-  consistent_waits o t1 ->
+  consistent_waits o t1      ->
   t1 --[e_read ad' t']--> t2 ->
   consistent_waits o t2.
-Proof. solve_cwaits_preservation. Qed.
+Proof. solve_cw_preservation. Qed.
 
-Lemma cwaits_preservation_write : forall o t1 t2 ad' t',
-  consistent_waits o t1 ->
+Lemma cw_preservation_write : forall o t1 t2 ad' t',
+  consistent_waits o t1       ->
   t1 --[e_write ad' t']--> t2 ->
   consistent_waits o t2.
-Proof. solve_cwaits_preservation. Qed.
+Proof. solve_cw_preservation. Qed.
 
-Lemma cwaits_preservation_acq : forall o m t1 t2 ad' t',
-  value t'        ->
-  valid_term m t' ->
-  valid_waits  t' ->
-  valid_term m t1 ->
-  valid_waits  t1 ->
+Lemma cw_preservation_acq : forall o t1 t2 ad' t',
+  value t'                    ->
+  consistent_waits WR_none t' ->
+  keywords t1                 ->
   (* --- *)
   consistent_waits o t1     ->
   t1 --[e_acq ad' t']--> t2 ->
   consistent_waits o t2.
-Proof.
-  solve_cwaits_preservation.
-  eauto 7 using cwaits_subst,
-                nocrs_from_value, nocrs_subst,
-                vwaits_subst,
-                nowaits_from_value, rwaits_subst.
-Qed.
+Proof. solve_cw_preservation. Qed.
 
-Lemma cwaits_preservation_rel : forall o t1 t2 ad',
-  valid_waits t1  ->
-  (* --- *)
+Lemma cw_preservation_rel : forall o t1 t2 ad',
   consistent_waits o t1  ->
   t1 --[e_rel ad']--> t2 ->
   consistent_waits o t2.
-Proof. solve_cwaits_preservation. Qed.
+Proof. solve_cw_preservation. Qed.
 
-Lemma cwaits_preservation_wacq : forall o t1 t2 ad',
-  consistent_waits o t1  ->
+Lemma cw_preservation_wacq : forall o t1 t2 ad',
+  consistent_waits o t1   ->
   t1 --[e_wacq ad']--> t2 ->
   consistent_waits o t2.
-Proof. solve_cwaits_preservation. Qed.
+Proof. solve_cw_preservation. Qed.
 
-Lemma cwaits_preservation_wrel : forall o t1 t2 ad',
-  consistent_waits o t1  ->
+Lemma cw_preservation_wrel : forall o t1 t2 ad',
+  consistent_waits o t1   ->
   t1 --[e_wrel ad']--> t2 ->
   consistent_waits o t2.
-Proof. solve_cwaits_preservation. Qed.
+Proof. solve_cw_preservation. Qed.
 
-Lemma cwaits_preservation_spawn : forall o t1 t2 t',
-  consistent_waits o t1  ->
+Lemma cw_preservation_spawn : forall o t1 t2 t',
+  consistent_waits o t1   ->
   t1 --[e_spawn t']--> t2 ->
   consistent_waits o t2.
-Proof. solve_cwaits_preservation. Qed.
+Proof. solve_cw_preservation. Qed.
 
-Lemma cwaits_preservation_spawned : forall m t1 t2 t',
-  valid_term m t1 ->
-  valid_waits  t1 ->
-  (* --- *)
+Lemma cw_preservation_spawned : forall o t1 t2 t',
+  consistent_waits o t1   ->
   t1 --[e_spawn t']--> t2 ->
-  consistent_waits None t'.
-Proof.
-  eauto using nocrs_spawn_term, rwaits_spawn_term, cwaits_from_rwaits.
-Qed.
+  consistent_waits WR_none t'.
+Proof. solve_cw_preservation. Qed.
 
 (* ------------------------------------------------------------------------- *)
 
-Theorem cwaits_preservation_threads : forall m1 m2 ths1 ths2 tid e,
-  forall_memory  m1   value           ->
-  forall_memory  m1   (valid_term m1) ->
-  forall_memory  m1   valid_waits     ->
-  forall_threads ths1 (valid_term m1) ->
-  forall_threads ths1 valid_waits     ->
-  (* --- *)
-  forall_threads ths1 (consistent_waits None) ->
-  m1 \ ths1 ~~[tid, e]~~> m2 \ ths2           ->
-  forall_threads ths2 (consistent_waits None).
+Corollary cw_preservation_memory : forall m1 m2 ths1 ths2 tid e,
+  forall_memory  m1   (consistent_waits WR_none) ->
+  forall_threads ths1 (consistent_waits WR_none) ->
+  m1 \ ths1 ~~[tid, e]~~> m2 \ ths2    ->
+  forall_memory  m2   (consistent_waits WR_none).
 Proof.
-  intros. invc_cstep; try invc_mstep; upsilon.
-  - eauto using cwaits_preservation_none.
-  - eauto using cwaits_preservation_alloc.
-  - eauto using cwaits_preservation_init.
-  - eauto using cwaits_preservation_read.
-  - eauto using cwaits_preservation_write.
-  - eauto using cwaits_preservation_acq.
-  - eauto using cwaits_preservation_rel.
-  - eauto using cwaits_preservation_wacq.
-  - eauto using cwaits_preservation_wrel.
-  - eauto using cwaits_preservation_spawn.
-  - eauto using cwaits_preservation_spawned.
+  intros. invc_cstep; try invc_mstep; trivial; intros ? ? ?;
+  upsilon; eauto using wrnone_init_term, wrnone_write_term.
+  omicron; upsilon; auto; eauto.
 Qed.
 
-Theorem cwaits_preservation_base : forall t,
-  no_crs         t ->
-  reserved_waits t ->
+Corollary cw_preservation_threads : forall m1 m2 ths1 ths2 tid e,
+  forall_memory  m1   value    ->
+  forall_threads ths1 keywords ->
   (* --- *)
-  forall_threads (base t) (consistent_waits None).
+  forall_memory  m1   (consistent_waits WR_none) ->
+  forall_threads ths1 (consistent_waits WR_none) ->
+  m1 \ ths1 ~~[tid, e]~~> m2 \ ths2              ->
+  forall_threads ths2 (consistent_waits WR_none).
 Proof.
-  auto using forallthreads_base, cwaits_from_rwaits, consistent_waits.
+  intros. invc_cstep; try invc_mstep; upsilon.
+  - eauto using cw_preservation_none.
+  - eauto using cw_preservation_alloc.
+  - eauto using cw_preservation_init.
+  - eauto using cw_preservation_read.
+  - eauto using cw_preservation_write.
+  - eauto using cw_preservation_acq.
+  - eauto using cw_preservation_rel.
+  - eauto using cw_preservation_wacq.
+  - eauto using cw_preservation_wrel.
+  - eauto using cw_preservation_spawn.
+  - eauto using cw_preservation_spawned.
 Qed.
+
+Theorem cw_preservation_cstep : forall m1 m2 ths1 ths2 tid e,
+  forall_memory  m1      value    ->
+  forall_program m1 ths1 keywords ->
+  (* --- *)
+  forall_program m1 ths1 (consistent_waits WR_none) ->
+  m1 \ ths1 ~~[tid, e]~~> m2 \ ths2                 ->
+  forall_program m2 ths2 (consistent_waits WR_none).
+Proof.
+  intros * ? [_ ?] [? ?] ?. split;
+  eauto using cw_preservation_memory, cw_preservation_threads.
+Qed.
+
