OneCR.v
@@ -60,6 +60,8 @@ Inductive one_cr (ad : addr) : tm -> Prop :=
   | onecr_cr_neq : forall ad' t,    ad <> ad'    ->
                                     one_cr ad t  ->
                                     one_cr ad <{cr ad' t                 }>
+  | onecr_wait   : forall t,        one_cr ad t  ->
+                                    one_cr ad <{wait t                   }>
   .
 
 (* inversion --------------------------------------------------------------- *)
@@ -83,6 +85,8 @@ Local Ltac _onecr tt :=
   | H : one_cr _ <{_ := _                }> |- _ => tt H
   | H : one_cr _ <{acq _ _ _             }> |- _ => tt H
   | H : one_cr _ <{cr _ _                }> |- _ => tt H
+  | H : one_cr _ <{wait _                }> |- _ => tt H
+  | H : one_cr _ <{reacq _               }> |- _ => inv H
   | H : one_cr _ <{spawn _               }> |- _ => inv H
   end.
 
@@ -97,7 +101,7 @@ Lemma onecr_subst : forall ad x tx t,
   one_cr ad <{[x := tx] t}>.
 Proof.
   intros. induction t; invc_onecr;
-  simpl; try destruct _str_eq_dec;
+  simpl; repeat destruct _str_eq_dec;
   auto using nocr_subst, one_cr.
 Qed.
 
@@ -180,13 +184,13 @@ Lemma onecr_preservation_alloc : forall ad t1 t2 ad' T',
   one_cr ad t2.
 Proof. solve_onecr_preservation nocr_preservation_alloc. Qed.
 
-Lemma onecr_preservation_insert : forall ad m t1 t2 ad' t',
+Lemma onecr_preservation_init : forall ad m t1 t2 ad' t',
   valid_term m t1 ->
   (* --- *)
   one_cr ad t1 ->
-  t1 --[e_insert ad' t']--> t2 ->
+  t1 --[e_init ad' t']--> t2 ->
   one_cr ad t2.
-Proof. solve_onecr_preservation nocr_preservation_insert. Qed.
+Proof. solve_onecr_preservation nocr_preservation_init. Qed.
 
 Lemma onecr_preservation_read : forall ad t1 t2 ad' t',
   no_crs t' ->
@@ -220,20 +224,23 @@ Lemma onecr_preservation_rel : forall ad t1 t2 ad',
   one_cr ad t2.
 Proof. solve_onecr_preservation nocr_preservation_rel. Qed.
 
-Lemma onecr_preservation_spawn : forall ad m t1 t2 tid t,
+Lemma onecr_preservation_spawn : forall ad m t1 t2 t',
   valid_term m t1 ->
   (* --- *)
   one_cr ad t1 ->
-  t1 --[e_spawn tid t]--> t2 ->
+  t1 --[e_spawn t']--> t2 ->
   one_cr ad t2.
 Proof. solve_onecr_preservation nocr_preservation_spawn. Qed.
 
 (* inheritance ------------------------------------------------------------- *)
 
 Local Ltac solve_onecr_inheritance L :=
-  intros; ind_tstep; repeat invc_vtm; try invc_onecr; eauto using L, one_cr;
-  try solve [exfalso; eauto using nocr_from_value, nocr_subst,
-    nocr_onecr_contradiction].
+  intros; ind_tstep; repeat invc_vtm; try invc_onecr; auto;
+  eauto using L, nocr_from_value, one_cr; exfalso;
+  match goal with H : one_cr ?ad ?t |- _ =>
+    apply (nocr_onecr_contradiction ad t);
+    eauto using nocr_from_value, nocr_subst, no_cr
+  end.
 
 Lemma onecr_inheritance_none : forall ad m t1 t2,
   valid_term m t1 ->
@@ -241,10 +248,7 @@ Lemma onecr_inheritance_none : forall ad m t1 t2,
   one_cr ad t2 ->
   t1 --[e_none]--> t2 ->
   one_cr ad t1.
-Proof.
-  solve_onecr_inheritance nocr_inheritance_none.
-  eapply onecr_seq2; eauto using nocr_from_value.
-Qed.
+Proof. solve_onecr_inheritance nocr_inheritance_none. Qed.
 
 Lemma onecr_inheritance_alloc : forall ad t1 t2 ad' T',
   one_cr ad t2 ->
@@ -252,13 +256,13 @@ Lemma onecr_inheritance_alloc : forall ad t1 t2 ad' T',
   one_cr ad t1.
 Proof. solve_onecr_inheritance nocr_inheritance_alloc. Qed.
 
-Lemma onecr_inheritance_insert : forall ad m t1 t2 ad' t',
+Lemma onecr_inheritance_init : forall ad m t1 t2 ad' t',
   valid_term m t1 ->
   (* --- *)
   one_cr ad t2 ->
-  t1 --[e_insert ad' t']--> t2 ->
+  t1 --[e_init ad' t']--> t2 ->
   one_cr ad t1.
-Proof. solve_onecr_inheritance nocr_inheritance_insert. Qed.
+Proof. solve_onecr_inheritance nocr_inheritance_init. Qed.
 
 Lemma onecr_inheritance_read : forall ad t1 t2 ad' t',
   no_crs t' ->
@@ -293,11 +297,11 @@ Lemma onecr_inheritance_rel : forall ad t1 t2 ad',
   one_cr ad t1.
 Proof. solve_onecr_inheritance nocr_inheritance_rel. Qed.
 
-Lemma onecr_inheritance_spawn : forall ad m t1 t2 tid t,
+Lemma onecr_inheritance_spawn : forall ad m t1 t2 t',
   valid_term m t1 ->
   (* --- *)
   one_cr ad t2 ->
-  t1 --[e_spawn tid t]--> t2 ->
+  t1 --[e_spawn t']--> t2 ->
   one_cr ad t1.
 Proof. solve_onecr_inheritance nocr_inheritance_spawn. Qed.
 
