InheritanceNoCR.v
@@ -10,7 +10,7 @@ Local Lemma nocr_inheritance_subst : forall x Tx t tx ad,
 Proof.
   intros. repeat constructor; trivial.
   induction t; simpl in *;
-  try destruct _str_eq_dec; try invc_nocr; auto using no_cr.
+  repeat destruct _str_eq_dec; try invc_nocr; auto using no_cr.
 Qed.
 
 (* ------------------------------------------------------------------------- *)
@@ -33,11 +33,11 @@ Lemma nocr_inheritance_alloc : forall ad t1 t2 ad' T',
   no_cr ad t1.
 Proof. solve_nocr_inheritance. Qed.
 
-Lemma nocr_inheritance_insert : forall ad m t1 t2 ad' t',
+Lemma nocr_inheritance_init : forall ad m t1 t2 ad' t',
   valid_term m t1 ->
   (* --- *)
   no_cr ad t2 ->
-  t1 --[e_insert ad' t']--> t2 ->
+  t1 --[e_init ad' t']--> t2 ->
   no_cr ad t1.
 Proof. solve_nocr_inheritance. Qed.
 
@@ -70,11 +70,24 @@ Lemma nocr_inheritance_rel : forall ad t1 t2 ad',
   no_cr ad t1.
 Proof. solve_nocr_inheritance. Qed.
 
-Lemma nocr_inheritance_spawn : forall ad m t1 t2 tid t,
+Lemma nocr_inheritance_wacq : forall ad t1 t2 ad',
+  no_cr ad t2 ->
+  t1 --[e_wacq ad']--> t2 ->
+  no_cr ad t1.
+Proof. solve_nocr_inheritance. Qed.
+
+Lemma nocr_inheritance_wrel : forall ad t1 t2 ad',
+  ad <> ad' ->
+  no_cr ad t2 ->
+  t1 --[e_wrel ad']--> t2 ->
+  no_cr ad t1.
+Proof. solve_nocr_inheritance. Qed.
+
+Lemma nocr_inheritance_spawn : forall ad m t1 t2 t',
   valid_term m t1 ->
   (* --- *)
   no_cr ad t2 ->
-  t1 --[e_spawn tid t]--> t2 ->
+  t1 --[e_spawn t']--> t2 ->
   no_cr ad t1.
 Proof. solve_nocr_inheritance. Qed.
 
